src/tls/TLS.fst
@@ -643,16 +643,16 @@ val next_fragment: i:id -> c:connection -> ST (result (TLS.Handshake.Send.outgoi
 let next_fragment i c =
   let s = c.hs in
   let h0 = get() in
-  let n = Machine.nonce s in 
-  let ilog = (Machine.epochs s n).es in
   let w0 = Handshake.i s Writer in
+(*
   let _  = if w0 >= 0
 	   then (MS.i_at_least_is_stable w0 (MS.i_sel h0 ilog).(w0) ilog;
 		 FStar.Seq.contains_intro (MS.i_sel h0 ilog) w0 (MS.i_sel h0 ilog).(w0);
 	         ST.mr_witness ilog (MS.i_at_least w0 (MS.i_sel h0 ilog).(w0) ilog)) in
+*)
   trace ("HS.next_fragment "^(if ID12? i then "ID12" else (if ID13? i then "ID13" else "PlaintextID"))^"?");
   let res = Handshake.next_fragment s i in
-  if w0 >= 0 then ST.testify (MS.i_at_least w0 (MS.i_sel h0 ilog).(w0) ilog);
+//  if w0 >= 0 then ST.testify (MS.i_at_least w0 (MS.i_sel h0 ilog).(w0) ilog);
   res
 
 
